Added typing rules for Pallene
Added a type judgment and a type algorithm for Pallene, plus
a proof that they define the same types.

pallene.v
@@ -6,6 +6,8 @@ Require Import Bool.
 Require Import Nat.
 Require Import Lia.
 
+Require Import LIR.maps.
+
 Require Import LIR.lir.
 
 
@@ -15,18 +17,179 @@ Inductive TPall : Set :=
 .
 
 
+Fixpoint TPeq (t1 t2 : TPall) : bool :=
+  match t1, t2 with
+  | TPstar, TPstar => true
+  | TPnil, TPnil => true
+  | TPint, TPint => true
+  | TParr t1', TParr t2' => TPeq t1' t2'
+  | TPfun t1' t1'', TPfun t2' t2'' => TPeq t1' t2' && TPeq t1'' t2''
+  | _, _ => false
+  end.
+
+
+Lemma dec_TP : forall (t1 t2 : TPall), TPeq t1 t2 = true <-> t1 = t2.
+Proof.
+  split.
+  - generalize dependent t2.
+    induction t1; intros t2 H; destruct t2 eqn:?; try easy.
+    + f_equal. auto.
+    + simpl in H.  apply andb_prop in H.
+      destruct H. f_equal; auto.
+  - intros H; subst. induction t2; trivial.
+    simpl. auto using andb_true_intro.
+Qed.
+
+
+Lemma TPeqRefl : forall t, TPeq t t = true.
+Proof. intros t. apply dec_TP. trivial. Qed.
+
+
+Definition Environment := Map TPall.
+
 Inductive EPall : Set :=
 | EPnil : EPall
 | EPnum : nat -> EPall
 | EPplus : EPall -> EPall -> EPall
-| EPcntr : TPall -> EPall
-| EPindx : EPall -> EPall -> EPall
-| EPassg : EPall -> EPall -> EPall -> EPall
+| EPnew : TPall -> EPall
+| EPget : EPall -> EPall -> EPall
+| EPset : EPall -> EPall -> EPall -> EPall
 | EPvar : string -> EPall
-| EPcall :  EPall -> EPall -> EPall
+| EPapp :  EPall -> EPall -> EPall
 | EPfunc : string -> TPall -> EPall -> EPall
 | EPcast : EPall -> TPall -> EPall
 .
+
+
+Reserved Notation "Γ '|=' e ':' t"  (at level 40, no associativity,
+                                     e at next level).
+
+Inductive PTyping : Environment -> EPall -> TPall -> Prop :=
+| TyPnil : forall Γ, Γ |= EPnil : TPnil
+| TyInt : forall Γ n, Γ |= EPnum n : TPint
+| TyVal : forall Γ var T,
+    In Γ var = Some T ->
+    Γ |= EPvar var : T
+| TyAdd : forall Γ e1 e2,
+    Γ |= e1 : TPint ->
+    Γ |= e2 : TPint ->
+    Γ |= EPplus e1 e2 : TPint
+| TyNew : forall Γ T, Γ |= EPnew T : TParr T
+| TyGet : forall Γ e1 T e2,
+    Γ |= e1 : TParr T ->
+    Γ |= e2 : TPint ->
+    Γ |= EPget e1 e2 : T
+| TySet : forall Γ e1 T e2 e3,
+    Γ |= e1 : TParr T ->
+    Γ |= e2 : TPint ->
+    Γ |= e3 : T ->
+    Γ |= EPset e1 e2 e3 : T
+| TyFun : forall Γ var Tvar body Tbody,
+    var |=> Tvar; Γ |= body : Tbody ->
+    Γ |= EPfunc var Tvar body : TPfun Tvar Tbody
+| TyApp : forall Γ e1 e2 T1 T2,
+    Γ |= e1 : TPfun T1 T2 ->
+    Γ |= e2 : T1 ->
+    Γ |= EPapp e1 e2 : T2
+| TyCast : forall Γ e T1 T2,
+    Γ |= e : T1 ->
+    Γ |= EPcast e T2 : T2
+
+where "Γ '|=' e ':' t" := (PTyping Γ e t)
+.
+
+
+Fixpoint typeOf Γ e : option TPall :=
+  match e with
+  | EPnil => Some TPnil
+  | EPnum _ => Some TPint
+  | EPplus e1 e2 =>
+    match (typeOf Γ e1), (typeOf Γ e2) with
+    | Some TPint, Some TPint => Some TPint
+    | _, _ => None
+    end
+  | EPnew T => Some (TParr T)
+  | EPget e1 e2 =>
+    match (typeOf Γ e1), (typeOf Γ e2) with
+    | Some (TParr T), Some TPint => Some T
+    | _, _ => None
+    end
+  | EPset e1 e2 e3 =>
+    match (typeOf Γ e1), (typeOf Γ e2), (typeOf Γ e3) with
+    | Some (TParr T), Some TPint, Some T' =>
+        if TPeq T T' then Some T' else None
+    | _, _, _ => None
+    end
+  | EPvar var => In Γ var
+  | EPapp e1 e2 =>
+    match typeOf Γ e1, typeOf Γ e2 with
+    | Some (TPfun T1 T2), Some T1' =>
+        if TPeq T1 T1' then Some T2 else None
+    | _, _ => None
+    end
+  | EPfunc var Tv e =>
+    match typeOf (var |=> Tv; Γ) e with
+    | Some Tb => Some (TPfun Tv Tb)
+    | None => None
+    end
+  | EPcast e T =>
+    match typeOf Γ e with
+    | Some _ => Some T
+    | None => None
+    end
+  end.
+
+
+
+Lemma typeOfCorrect' : forall Γ e T, Γ |= e : T -> typeOf Γ e = Some T.
+Proof.
+  intros Γ e T Hty.
+  induction Hty; try easy;
+  simpl;
+  repeat match goal with
+  | [H: typeOf _ _ = Some _ |- _] => rewrite H; clear H end;
+  try easy; rewrite TPeqRefl; trivial.
+Qed.
+
+Ltac destTOf Γ e :=
+    destruct (typeOf Γ e) as [[ | | | ? | ? ?] | ?] eqn:?; try easy.
+
+Lemma typeOfCorrect'' : forall Γ e T, typeOf Γ e = Some T -> Γ |= e : T.
+Proof.
+  intros Γ e T Heq.
+  generalize dependent Γ.
+  generalize dependent T.
+  induction e; intros T Γ Heq; subst;
+  simpl in Heq; inversion Heq; subst; eauto using PTyping.
+  - destTOf Γ e1.
+    destTOf Γ e2.
+    inversion Heq; subst. eauto using PTyping.
+  - destTOf Γ e1.
+    destTOf Γ e2.
+    inversion Heq; subst. eauto using PTyping.
+  - destTOf Γ e1.
+    destTOf Γ e2.
+    destruct (typeOf Γ e3) eqn:?; try easy.
+    destruct (TPeq t t0) eqn:?; try easy.
+    inversion Heq; subst.
+    assert(t = T). { apply dec_TP. trivial. }
+    subst. eauto using PTyping.
+  - destTOf Γ e1.
+    destruct (typeOf Γ e2) eqn:?; try easy.
+    destruct (TPeq t t1) eqn:?; try easy.
+    inversion Heq; subst. econstructor.
+    eapply IHe1. eauto.
+    assert (t = t1). { apply dec_TP. trivial. }
+    subst. auto.
+  - destruct (typeOf (s |=> t; Γ) e) eqn:?; try easy.
+    inversion Heq; subst. eauto using PTyping.
+  - destruct (typeOf Γ e) eqn:?; try easy.
+    inversion Heq; subst. eauto using PTyping.
+Qed.
+
+Theorem typeOfCorrect : forall Γ e T, typeOf Γ e = Some T <-> Γ |= e : T.
+Proof. split; auto using typeOfCorrect', typeOfCorrect''. Qed.
+
 
 
 Fixpoint TP2FCT (t : TPall) : FCType :=
@@ -47,7 +210,35 @@ Fixpoint Cast (t1 t2 : FCType) (e : LirExp) : LirExp :=
   | Ttag t1', Ttag t2' => if dec_Tag t1' t2' then e
                             else Ebox t1' (Eunbox t2' e)
   end.
- 
+
+
+Notation "'<' t1 '<=' t2 '>' e" := (Cast t1 t2 e)
+    (at level 50, t1 at next level, t2 at next level).
+
+(*
+Definition Pall2Lir (Γ : Environment) (e : EPall) (t : TPall)
+  (Hty : Γ |= e : t) : LirExp.
+refine ((fix Pall2Lir (Γ : Environment) (e : EPall) (t : TPall)
+  (Hty : Γ |= e : t) {struct e}  : LirExp :=
+    (match e as e0 return (e = e0 -> LirExp) with
+    | EPnil => fun Heq => Enil
+    | EPnum a => fun Heq => Enum a
+    | EPplus e1 e2 => fun Heq =>
+         Eplus (Pall2Lir _ e1 _ _) (Pall2Lir _ e2 _ _)
+    | EPnew _ => fun Heq => Ecstr
+    | EPget e1 e2 => fun Heq =>
+         <(TP2FCT t) <= Tstar> (Eindx (Pall2Lir _ e1 _ _)
+                                      (Pall2Lir _ e2 _ _))
+    | EPset e1 e2 e3 => fun Heq =>
+         (Eassg (Pall2Lir _ e1 _ _)
+               (Pall2Lir _ e2 _ _)
+               (<Tstar <= (TP2FCT t)> Pall2Lir _ e3 _ _))
+    | EPcast e t1 t2 => fun Heq =>
+         <(TP2FCT t2) <= (TP2FCT t1)> (Pall2Lir _ e _ _)
+    | _ => fun Heq => Enil
+    end) (eq_refl e)) Γ e t Hty);
+ subst; inversion Hty; subst; eauto.
+
 
 Fixpoint Pall2Lir (e : EPall) : LirExp :=
   match e with
@@ -55,11 +246,14 @@ Fixpoint Pall2Lir (e : EPall) : LirExp :=
   | EPnum a => Enum a
   | EPplus e1 e2 => Eplus (Pall2Lir e1) (Pall2Lir e2)
   | EPcntr => Ecstr
-  | EPindx e1 e2 =>  Eindx (Pall2Lir e1) (Pall2Lir e2)
-  | EPassg e1 e2 e3 : Eassg  (Pall2Lir e1) (Pall2Lir e2) (Pall2Lir e3)
+  | EPget e1 e2 =>  Eindx (Pall2Lir e1) (Pall2Lir e2)
+  | EPset e1 e2 e3 : Eassg  (Pall2Lir e1) (Pall2Lir e2) (Pall2Lir e3)
   | EPvar v => Evar v
-  | EPcall :w
+  | EPapp :w
 :  EPall -> EPall -> EPall
   | EPfunc : string -> TPall -> EPall -> EPall
   | EPcast : EPall -> TPall -> EPall
   end.
+
+*)
+
